% TeX root = ../Main.tex

% First argument to \section is the title that will go in the table of contents. Second argument is the title that will be printed on the page.
\section[Lecture 16 (Nov 6) -- {\it Decision Theory}]{Lecture 16}

\subsection{Decision theory basics}

\begin{db}
Define a loss function:
\[
\mathcal{L}(\theta,\hat \theta): (\Theta \times \mathcal{A}) \to [0,\infty)
\]
e.g. squared error loss:
$\mathcal{L}(\theta,\hat \theta) = (\theta - \hat \theta)^2$

\textbf{Risk} (Average loss over all possible data) a.k.a. frequentist risk:
\[
R(\theta,\hat \theta) = \mathbb{E}_{X|\theta} \left[ \mathcal{L}(\theta,\hat \theta(X)) \right] = \int \mathcal{L}(\theta,\hat \theta(x)) f(x|\theta) dx
\]
\textbf{Posterior risk} (Average loss over posterior distribution of $\theta$):
\[
r(\hat \theta | \mathbf{x}) = E_{\theta | \bf{x}}  \left[ \mathcal{L}(\theta,\hat \theta) \right] = \int \mathcal{L}(\theta,\hat \theta) f(\theta | \bf{x}) d\theta
\]

where $\mathbf{x} \triangleq (x_1,\dots,x_n)$
\end{db}

\begin{eb}
Prior: $X_1,\dots,X_n \iid N(\theta,1), \qquad f(\theta) \sim N(0,\tau^2)$

\[
f(\theta|\mathbf{x}) \propto \exp\{- \dfrac{\sum\limits_{i=1}^{n} (x_i - \theta)^2}{2}\} \exp\{- \dfrac{\theta^2}{2\tau^2}\} \propto \exp\{- \dfrac{1}{2} \left( (n + \dfrac{1}{\tau^2}) \theta^2 - 2n\bar{x} \theta \right) \}
\]
\[
\theta | x \sim N(\dfrac{n\tau^2}{n\tau^2 + 1} \bar X_n, \dfrac{\tau^2}{n\tau^2 + 1})
\]

\[
r(\hat \theta | x)  = E_{\theta|x} (\theta - \hat \theta)^2
= E_{\theta |x} (\theta^2) - 2 \hat \theta \cdot E_{\theta | x} (\theta) +\hat \theta^2
\]
\[
= -(\hat \theta - \frac{n\tau^2}{n\tau^2 + 1}\bar X_n)^2 + \dfrac{\tau^2}{n\tau^2 + 1} 
\]

Posterior risk is minimized at $\hat \theta = E[\theta | x] = \dfrac{n\tau^2}{n\tau^2 + 1} \bar X_n$


\end{eb}

\begin{eb}[Frequentist risk]
\[
\mathcal{L} (\theta, \hat \theta) = (\theta - \hat \theta)^2 
\]

\[
R(\theta ,\hat \theta ) = E_{x|\theta} (\hat \theta)^2 - 2\theta \cdot E_{x|\theta} (\hat \theta) + \theta^2
\]
\[
= Var_{x|\theta}(\hat \theta) + (E_{x|\theta}(\hat \theta) - \theta)^2 = MSE(\hat \theta)
\]
\end{eb}

Consider two estimators, $\hat{\theta}$ and $\hat{\theta}'$. 
We say $\hat{\theta}'$ \textbf{dominates} $\hat{\theta}$ if
\[
R(\theta, \hat{\theta}') \le R(\theta, \hat{\theta}) \quad \text{for all } \theta,
\]
and
\[
R(\theta, \hat{\theta}') < R(\theta, \hat{\theta}) \quad \text{for at least one } \theta.
\]

The estimator $\hat{\theta}$ is called \textbf{inadmissible} if there is at least one other estimator 
$\hat{\theta}'$ that dominates it. Otherwise it is called \textbf{admissible}.


\begin{db}[Bayes risk]
The Bayes risk is defined as:

\[
\begin{aligned}
r(f, \hat{\theta}) 
&= \int \underbrace{R(\theta, \hat{\theta})}_{\text{frequentist risk}} f(\theta)\, d\theta \\[6pt]
&= \int \left[ \int L(\theta, \hat{\theta}(x)) f(x \mid \theta)\, dx \right] f(\theta)\, d\theta \\[6pt]
&= \int \!\!\int L(\theta, \hat{\theta}(x)) f(x, \theta)\, dx\, d\theta \\[6pt]
&= \int \left[ \int L(\theta, \hat{\theta}(x)) f(\theta \mid x)\, d\theta \right] f(x)\, dx \\[6pt]
&= \int \underbrace{r(\hat \theta \mid x)}_{\text{posterior risk}}\, f(x)\, dx
\end{aligned}
\]

\noindent
This expression averages over both $\theta$ and $X$. It depends on the particular form of $\hat{\theta}$,
and on the probability models for the data $f(x \mid \theta)$ and the parameter $\theta$ ($f(\theta)$).
\end{db}


\begin{eb}
\[
X \sim N(\theta, 1), \hat \theta_c (x) = cx, \theta \sim N(0,\tau^2), \mathcal{L}(\theta,\hat \theta) = (\theta - \hat \theta)^2 = (\theta - cX)^2
\]

\paragraph{Frequentist -> Integral over the parameter} % (fold)
\label{par:Frequentist -> Integral over the parameter}

\[
R(\theta,\hat \theta_c) = E_{x\mid \theta} (\theta -cx)^2 = (c - 1)^2 \theta^2 + c^2
\]

Bayes risk:
\[
r(f,\hat \theta_c) = \int R(\theta,\hat \theta_c) f(\theta) d\theta = (c - 1)^2 \tau^2 + c^2
\]

F.O.C. w.r.t. $c$:
\[
\implies c = \dfrac{\tau^2}{\tau^2 + 1}
\]

Thus, the Bayes rule is $\hat \theta_{\text{Bayes}} = \dfrac{\tau^2}{\tau^2 + 1} X$.
% paragraph Frequentist -> Integral over the parameter (end)

\paragraph{Bayesian -> Integral over the data} % (fold)
\label{par:Bayesian -> Integral over the data}

\[
f(\theta \mid x) \propto f(x | \theta) f(\theta) \propto \exp\{-\dfrac{(x - \theta)^2}{2}\} \exp\{- \dfrac{\theta^2}{2\tau^2}\} \propto \exp\{- \dfrac{1}{2} \left( (1 + \dfrac{1}{\tau^2}) \theta^2 - 2x \theta \right) \}
\]
Posterior distribution:
\[
\theta | x \sim N(\dfrac{\tau^2}{\tau^2 + 1} x, \dfrac{\tau^2}{\tau^2 + 1})
\]

Posterior risk:
\[
r(\hat \theta_c | x) = E_{\theta | x} (\theta - cx)^2 = (\dfrac{\tau^2}{\tau^2 + 1} - c)^2 x^2 + \dfrac{\tau^2}{\tau^2 + 1}
\] 
Posterior rule is $\hat \theta_c = \dfrac{\tau^2}{\tau^2 + 1}x$, and the posterior risk is $\dfrac{\tau^2}{\tau^2+1}$ at this value.

Thus, the posterior risk is invariant to $x$ at the posterior minimizing value.

The Bayes risk is:
\[
r(f,\hat \theta_c) = \int r(\hat \theta_c | x) f(x) dx = \dfrac{\tau^2}{\tau^2 + 1}
\]
% paragraph Bayesian -> Integral over the data (end)
\end{eb}